Updates to LinkedList and LinkedListSeg.

examples/LinkedListSeg.v
@@ -18,13 +18,8 @@ Record Node : Set := node {
   next: LinkedList
 }.
 
-Definition ptr_eq : forall (p q : ptr), {p = q} + {p <> q}.
-  decide equality.
-Qed.
-
-Definition ptr_eq' : forall (p q : option ptr), {p = q} + {p <> q}.
-  decide equality; apply ptr_eq.
-Qed.
+Parameter ptr_eq : forall (p q : ptr), {p = q} + {p <> q}.
+Parameter ptr_eq' : forall (p q : option ptr), {p = q} + {p <> q}.
 
 Definition head (ls : list A) :=
   match ls with
@@ -37,6 +32,19 @@ Definition tail (ls : list A) :=
     | nil => nil
     | _ :: ls' => ls'
   end.
+(**
+Fixpoint llseg (s : LinkedList) (e : LinkedList) (m : list A) {struct m} : hprop :=
+  match m with 
+    | nil    => [s = e]
+    | v :: r => match s with
+                  | None => [False]
+                  | Some p => match e with
+                                | None   => Exists nde :@ Node, p --> nde * [v = data nde] * llseg (next nde) None r
+                                | Some q => [q <> p] * Exists nde :@ Node, p --> nde * [v = data nde] * llseg (next nde) e r
+                              end
+                end
+  end.
+**)
 
 Fixpoint llseg (s : LinkedList) (e : LinkedList) (m : list A) {struct m} : hprop :=
   match m with 
@@ -58,9 +66,47 @@ Ltac simplr := repeat (try discriminate;
 (**    | [ |- context[?X None None ?L] ] => destruct L **)
   end).
 
-Ltac t := unfold llist; unfold llseg; sep simplr.
+Theorem llist_unfold : forall ls hd,
+  llist hd ls ==> llseg hd None ls.
+  unfold llist; sep fail simpl.
+Qed.
+
+Theorem llseg_unfold_nil : forall hd tl,
+  llseg hd tl nil ==> [hd = tl].
+  unfold llseg; sep fail simpl.
+Qed.
+
+(**
+Theorem llseg_unfold_cons : forall hd tl ls v,
+  llseg hd tl (v :: ls) ==> Exists p :@ ptr, Exists nde :@ Node, [hd = Some p] *
+    p --> nde * [v = data nde] * llseg (next nde) tl ls.
+  unfold llseg; destruct ls; destruct hd; destruct tl; sep fail simpl. 
+Qed.
+**)
+(**
+Theorem llseg_unfold : forall hd tl ls,
+  llseg hd tl ls ==> 
+  match ls with
+    | nil => [hd = tl]
+    | v :: r => (*[hd <> tl] *) match hd with
+                               | None => [False]
+                               | Some p => Exists nde :@ Node, p --> nde * [v = data nde] * llseg (next nde) tl r
+                             end
+  end.
+  unfold llseg; destruct ls; destruct hd; sep fail simpl.
+Qed.
+
+Ltac simpl_prem :=
+  simpl_IfNull;
+  simpl_prem ltac:(apply llist_unfold || apply llseg_unfold_nil || apply llseg_unfold_cons || apply llseg_unfold).
+**)
+
+Ltac t := unfold llist; unfold llseg; sep fail simplr.
 Ltac f := fold llseg; fold llist.
 
+(********************)
+(** Implementation **)
+(********************)
 Definition empty : STsep __ (fun r:LinkedList => llseg r r nil).
   refine ({{Return None}});
     t. 
@@ -70,8 +116,14 @@ Definition cons : forall (v : A) (r : LinkedList) (q : [LinkedList]) (m : [list 
   STsep (q ~~ m ~~ llseg r q m)
         (fun r:LinkedList => q ~~ m ~~ llseg r q (v :: m)).
   intros;
-  refine (l <- New (node v r); {{Return (Some l)}}).
-Admitted.
+  refine (l <- New (node v r) <@> (m ~~ q ~~ llseg r q m); {{Return (Some l)}}).
+  t. t. t. 
+
+
+ t.  f. destruct x0. t. f.
+
+destruct x. destruct x0. t.
+Qed.
 
 Definition single : forall (v : A),
   STsep __ (fun r:LinkedList => llseg r None (v :: nil)).
@@ -110,20 +162,25 @@ Definition copy : forall (p' : LinkedList) (q : LinkedList) (ls' : [list A]),
         Else
           Assert (ls ~~ Exists nde :@ Node, [Some p <> q] * p --> nde * [head ls = Some (data nde)] * llseg (next nde) q (tail ls));;
           nde <- !p;
-          rr <- self (next nde) (ls ~~~ tail ls) <@> (ls ~~ p --> nde * [head ls = Some (data nde)]);
+          rr <- self (next nde) (ls ~~~ tail ls) <@> (ls ~~ [Some p <> q] * p --> nde * [head ls = Some (data nde)]);
           res <- cons (data nde) rr [q] (ls ~~~ tail ls) <@> (ls ~~ [Some p <> q] * p --> nde * [head ls = Some (data nde)] * llseg (next nde) q (tail ls));
           {{Return res}}) p' ls');
-  solve [ t | hdestruct ls; t ].
+  try solve [ t | hdestruct ls; t ].
+  t. destruct x. t. t.
 Qed.
 
-Fixpoint insertAt_model (ls : list A) (a : A) (idx : nat) {struct idx} : list A :=
-  match ls with 
+Fixpoint insertAt_model (ls : list A) (a : A) (idx : nat) {struct ls} : list A :=
+  match ls with
     | nil    => a :: ls
     | f :: r => match idx with
                   | 0 => a :: f :: r
                   | S idx' => f :: insertAt_model r a idx'
                 end
   end.
+
+Definition eq_nat : forall (a b : nat), {a = b} + {a <> b}.
+  decide equality.
+Qed.
 
 Definition insertAt : forall (p' : LinkedList) (a : A) (idx' : nat) (ls' : [list A]),
   STsep (ls' ~~ llist p' ls')
@@ -134,11 +191,25 @@ Definition insertAt : forall (p' : LinkedList) (a : A) (idx' : nat) (ls' : [list
     (fun p ls idx (r:LinkedList) => ls ~~ llist r (insertAt_model ls a idx))
     (fun self p ls idx =>
       IfNull p Then
-        
+        Assert (ls ~~ [ls = nil] * llist p nil);;
+        {{cons a p [None] ls <@> (ls ~~ [ls = nil])}}
       Else
-        _
+        Assert (ls ~~ [ls <> nil] * Exists nde :@ Node, p --> nde * [head ls = Some (data nde)] * llist (next nde) (tail ls));;
+        nde <- !p;
+        if eq_nat idx 0 then
+          r <- cons a (Some p) [None] ls <@> (ls ~~ p --> nde * [head ls = Some (data nde)]);
+          p ::= node (data nde) r;;
+          {{Return (Some p)}}
+        else 
+          nde <- !p;
+          {{self (next nde) (ls ~~~ tail ls) (pred idx)}}
       ) p' ls' idx').
+  hdestruct ls; t.
   t.
+  t.
+  t.
+  t.
+  
   
 
 Definition append : forall (p' : LinkedList) (q : LinkedList)
